lean/Vsr.lean
@@ -8,3 +8,4 @@ import Vsr.Liveness
 import Vsr.Check
 import Vsr.Safety
 import Vsr.Invariant
+import Vsr.Preserve
